KHasTy

Gt3/HasTy/Basic.lean
@@ -28,7 +28,7 @@ inductive Ctx.HasTy : Ctx → Tm 0 → Tm 0 → Prop
     (hA : HasTy Γ (.univ m) A) (hB : ∀ x ∉ L, HasTy (Γ.cons x A) (.univ n) (B.open x))
     (hm : m ≤ ℓ) (hn : n ≤ ℓ) (hℓ : 1 ≤ ℓ)
     : HasTy Γ (.univ ℓ) (.sigma A B)
-  | pair {Γ} {A a b : Tm 0} {B : Tm 1} {m n : ℕ} {L : Finset String}
+  | pair' {Γ} {A a b : Tm 0} {B : Tm 1} {m n : ℕ} {L : Finset String}
     (hA : HasTy Γ (.univ m) A) (hB : ∀ x ∉ L, HasTy (Γ.cons x A) (.univ n) (B.open x))
     (ha : HasTy Γ A a) (hb : HasTy Γ (B.lst a) b)
     : HasTy Γ (.sigma A B) (.pair a b)
